Function description contains uncurried model function instead of curried

library/modelled.v
@@ -8,40 +8,6 @@ Import ListNotations.
 Require Import VeriFFI.library.isomorphism.
 Require Import VeriFFI.library.meta.
 
-Ltac eq_refl_match :=
-  match goal with
-  | [ |- context[match ?x with | eq_refl => _ end] ] => destruct x
-  (* | [ _ : context[match ?x with | eq_refl => _ end] |- _] => destruct x *)
-  end.
-
-Ltac prim_rewrites :=
-  repeat eq_refl_match;
-  repeat rewrite ?from_to, ?to_from.
-
-Ltac props x :=
-  let P := fresh in
-  pose proof x as P;
-  hnf in P;
-  simpl in P;
-  rewrite !P;
-  unfold id, eq_rect in *;
-  clear P.
-
-(* opaque and transparent *)
-(* Inductive annotated : Type := *)
-(* | TYPEPARAM : (forall (A : Type) `{InGraph A}, annotated) -> annotated *)
-(* | OPAQUE : forall (prim_type model_type : Type) *)
-(*                     `{Isomorphism prim_type model_type}, *)
-(*                     (option (prim_type -> annotated)) -> *)
-(*                     annotated *)
-(* | TRANSPARENT : forall (A : Type) `{InGraph A}, (option (A -> annotated)) -> annotated. *)
-
-
-(* Inductive prim_ann (actual_type : Type) `(InGraph actual_type) : Type := *)
-(* | OPAQUE : forall (model_type : Type) `{InGraph actual_type}, `{Isomorphism actual_type model_type} -> prim_ann actual_type *)
-(* | TRANSPARENT : `{InGraph actual_type} -> prim_ann actual_type. *)
-
-
 Class prim_ann (primary : Type) : Type :=
   { prim_in_graph : InGraph primary
   ; secondary : Type
@@ -63,15 +29,6 @@ Definition opaque {A : Type} (B : Type)
 
 Definition prim_ann_any {A} : prim_ann A := @transparent A InGraph_any.
 
-Fixpoint to_model_fn_type (r : reified prim_ann) : Type :=
-  match r with
-  | TYPEPARAM f =>
-      forall (A : Type) (H : prim_ann A),
-        to_model_fn_type (f A H)
-  | ARG primary ann k => forall (p : primary), to_model_fn_type (k p)
-  | RES primary ann => primary
-  end.
-
 Fixpoint to_prim_fn_type (r : reified prim_ann) : Type :=
   match r with
   | TYPEPARAM f =>
@@ -81,6 +38,17 @@ Fixpoint to_prim_fn_type (r : reified prim_ann) : Type :=
       forall (m : secondary),
         to_prim_fn_type (k (@to primary secondary prim_iso m))
   | RES _ ann => secondary
+  end.
+
+(*
+(* Old version with extra parameter: *)
+Fixpoint to_model_fn_type (r : reified prim_ann) : Type :=
+  match r with
+  | TYPEPARAM f =>
+      forall (A : Type) (H : prim_ann A),
+        to_model_fn_type (f A H)
+  | ARG primary ann k => forall (p : primary), to_model_fn_type (k p)
+  | RES primary ann => primary
   end.
 
 Fixpoint uncurry (r : reified prim_ann)
@@ -99,17 +67,44 @@ Proof.
     auto.
   * auto.
 Defined. 
+*)
+
+Fixpoint to_model_fn_type (r : reified prim_ann) : Type :=
+  match r with
+  | TYPEPARAM f =>
+      forall (A : Type),
+        to_model_fn_type (f A prim_ann_any)
+  | ARG primary ann k => forall (p : primary), to_model_fn_type (k p)
+  | RES primary ann => primary
+  end.
+
+Fixpoint curry_model_fn
+         (r : reified prim_ann)
+         (mt : reflect r) {struct r} : to_model_fn_type r.
+Proof.
+  unfold reflect in *.
+  destruct r.
+  * intro A.
+    refine (curry_model_fn (r A prim_ann_any) (fun P => _)).
+    change (projT1 (result (TYPEPARAM prim_ann r) (A; (prim_ann_any; P)))).
+    apply mt.
+  * intro a.
+    refine (curry_model_fn (r a) (fun P => _)).
+    change (projT1 (result (ARG prim_ann A r) (a; P))).
+    apply mt.
+  * exact (mt tt).
+Defined.
 
 Record fn_desc :=
   { type_desc : reified prim_ann
   ; prim_fn : to_prim_fn_type type_desc
-  ; model_fn : to_model_fn_type type_desc
+  ; model_fn : reflect type_desc
   ; f_arity : nat
   ; c_name : string
   }.
 
-Definition uncurried_model_fn (d : fn_desc) : reflect (type_desc d) :=
-  uncurry (type_desc d) (model_fn d).
+Definition curried_model_fn (d : fn_desc) : to_model_fn_type (type_desc d) :=
+  curry_model_fn (type_desc d) (model_fn d).
 
 (*
 From Equations Require Import Equations Signature.
@@ -127,11 +122,10 @@ Equations model_spec_aux
 model_spec_aux (@TYPEPARAM f) pt mt :=
   forall (A : Type), model_spec_aux (f A prim_ann_any) (pt A) (mt A) ;
 model_spec_aux (@ARG primary ann k) pt mt :=
-  forall (x : primary),
-    model_spec_aux (k x) (pt x)
-      (ltac: (rewrite_apply (@from_to _ _ prim_iso) (mt (@from _ _ prim_iso x)))) ;
+  forall (x : secondary),
+    model_spec_aux (k (to x)) (pt x) (mt (to x)) ;
 model_spec_aux (@RES primary ann) pt mt :=
-  pt = @to _ _ prim_iso mt.
+  pt = @from _ _ prim_iso mt.
 *)
 
 Fixpoint model_spec_aux
@@ -141,15 +135,32 @@ Fixpoint model_spec_aux
 Proof.
   destruct a as [f | primary ann k | A ann]; simpl in ft, mt.
   * exact (forall (A : Type),
-              model_spec_aux (f A prim_ann_any) (ft A) (mt A prim_ann_any)).
+              model_spec_aux (f A prim_ann_any) (ft A) (mt A)).
   * destruct ann as [IG secondary Iso].
     refine (forall (x : secondary), model_spec_aux (k (to x)) (ft x) (mt (to x))).
-    (* pose (m := ft (@from primary secondary _ x)). *)
-    (* rewrite from_to in m. *)
-    (* exact m. *)
   * destruct ann as [IG secondary Iso].
     exact (ft = from mt).
 Defined.
 
 Definition model_spec (d : fn_desc) : Prop :=
-  model_spec_aux (type_desc d) (prim_fn d) (model_fn d).
+  model_spec_aux (type_desc d) (prim_fn d) (curried_model_fn d).
+
+Ltac eq_refl_match :=
+  match goal with
+  | [ |- context[match ?x with | eq_refl => _ end] ] => destruct x
+  (* | [ _ : context[match ?x with | eq_refl => _ end] |- _] => destruct x *)
+  end.
+
+Ltac prim_rewrites :=
+  unfold curried_model_fn, curry_model_fn; simpl;
+  repeat eq_refl_match;
+  repeat rewrite ?from_to, ?to_from.
+
+Ltac props x :=
+  let P := fresh in
+  pose proof x as P;
+  hnf in P;
+  simpl in P;
+  rewrite !P;
+  unfold id, eq_rect in *;
+  clear P.
